ulib/FStar.Issue.fsti
@@ -1,6 +1,8 @@
 module FStar.Issue
 open FStar.Range
 
+module Pprint = FStar.Stubs.Pprint
+
 new
 val issue : Type0
 
@@ -11,7 +13,7 @@ let issue_level_string = s:string {
   s == "Feature not yet implemented: "
 }
 
-val message_of_issue (i:issue) : Tot string
+val message_of_issue (i:issue) : Tot (list Pprint.document)
 
 val level_of_issue (i:issue) : Tot issue_level_string
 
@@ -20,10 +22,28 @@ val number_of_issue (i:issue) : Tot (option int)
 val range_of_issue (i:issue) : Tot (option range)
 
 val context_of_issue (i:issue) : Tot (list string)
+
+val render_issue (i:issue) : Tot string
   
-val mk_issue (i:issue_level_string)
-             (msg:string)
+(* NOTE: the only way to build a document that actually reduces
+in interpreted mode (like in tactics when not using plugins)
+is using arbitrary_string, as below. *)
+val mk_issue_doc (i:issue_level_string)
+             (msg:list Pprint.document)
              (range:option range)
              (number:option int)
              (ctx:list string)
   : Tot issue
+
+(* These qualifiers here to make sure that karamel (while building
+krmllib) does not attempt to extract this definition, as that would fail
+since it does not have an implementation of arbitrary_string. We could
+also not extract this module altogether. *)
+noextract
+inline_for_extraction
+let mk_issue (i:issue_level_string)
+             (msg:string)
+             (range:option range)
+             (number:option int)
+             (ctx:list string)
+  = mk_issue_doc i [Pprint.arbitrary_string msg] range number ctx
